more simulation

Simulation.dfy
@@ -1,40 +1,62 @@
+// RUN: /compile:0 /nologo /noNLarith /noCheating:1 /rlimit:1000000
+
 module Spec {
     export reveals T, Behavior, BehaviorSatisfies
+           provides ExtendBehavior
 
-    datatype T<A> = Spec(init: iset<A>, next: iset<(A, A)>)
+    datatype T<A> = Make(init: iset<A>, next: iset<(A, A)>)
 
     type Behavior<A> = seq<A>
 
     predicate BehaviorSatisfies<A>(b: Behavior<A>, spec: T<A>)
     {
         && |b| > 0 ==> b[0] in spec.init
-        && forall i :: 0 <= i < |b| - 1 ==> (b[i], b[i+1]) in spec.next
+        && forall i, j ::
+            0 <= i < |b| - 1 && j == i + 1 ==> (b[i], b[j]) in spec.next
     }
+
+    lemma ExtendBehavior<A>(spec: T<A>, b: Behavior<A>, a: A)
+        requires |b| > 0 && BehaviorSatisfies(b, spec)
+        requires (b[|b| - 1], a) in spec.next
+        ensures  BehaviorSatisfies(b + [a], spec)
+    {}
 }
 
 
 module Simulation {
     import Spec
-    export reveals Request, ValidRequest
+    export reveals Request, InitDiagram, NextDiagram, ValidRequest
            provides Spec, PerformSimulation
-    
 
-    datatype Request<L, H> = 
+
+    datatype Request<L, H> =
         Request(
-          lspec: Spec.T<L>, 
-          hspec: Spec.T<H>, 
+          lspec: Spec.T<L>,
+          hspec: Spec.T<H>,
           sim_rel: iset<(L, H)>
           )
 
-    predicate ValidRequest<L, H>(req: Request<L, H>) 
+    predicate InitDiagram<L, H>(req: Request<L, H>)
     {
-        && (forall l :: l in req.lspec.init ==> exists h :: h in req.hspec.init && (l, h) in req.sim_rel)
-        && (forall l, l', h :: 
-            && (l, l') in req.lspec.next 
+        forall l :: l in req.lspec.init ==>
+            exists h ::
+                h in req.hspec.init && (l, h) in req.sim_rel
+    }
+
+    predicate NextDiagram<L, H>(req: Request<L, H>)
+    {
+        forall l, l', h ::
+            && (l, l') in req.lspec.next
             && (l, h) in req.sim_rel
-            ==> exists h' :: 
-                && (h, h') in req.hspec.next 
-                && (l', h') in req.sim_rel)
+            ==> exists h' ::
+                && (h, h') in req.hspec.next
+                && (l', h') in req.sim_rel
+    }
+
+    predicate ValidRequest<L, H>(req: Request<L, H>)
+    {
+        && InitDiagram(req)
+        && NextDiagram(req)
     }
 
     lemma PerformSimulation<L, H>(req: Request<L, H>, lb: Spec.Behavior<L>)
@@ -46,7 +68,7 @@ module Simulation {
         ensures forall i :: 0 <= i < |lb| ==> (lb[i], hb[i]) in req.sim_rel
     {
         hb := [];
-        while |hb| < |lb| 
+        while |hb| < |lb|
             invariant Spec.BehaviorSatisfies(hb, req.hspec)
             invariant 0 <= |hb| <= |lb|
             invariant forall i :: 0 <= i < |hb| ==> (lb[i], hb[i]) in req.sim_rel
@@ -57,6 +79,7 @@ module Simulation {
                 var h0 :| h0 in req.hspec.init && (lb[i+1], h0) in req.sim_rel;
                 h := h0;
             } else {
+                assert (lb[i], lb[i+1]) in req.lspec.next;
                 var h' :| (hb[i], h') in req.hspec.next && (lb[i+1], h') in req.sim_rel;
                 h := h';
             }
@@ -67,43 +90,129 @@ module Simulation {
 
 module Invariants {
     import Spec
-    export provides Spec, IsInvariant, EstablishInvariant
-           reveals IsInductive
+    export provides Spec, EstablishInvariantByInduction, InvariantTrueInitially
+           reveals IsInvariant, IsInductive
 
     predicate IsInductive<A>(inv: iset<A>, spec: Spec.T<A>)
     {
         && spec.init <= inv
-        && forall x, y :: 
-            && x in inv 
+        && forall x, y ::
+            && x in inv
             && (x, y) in spec.next
+            ==> y in inv
+    }
+
+    predicate IsInductiveInReachable<A>(inv: iset<A>, spec: Spec.T<A>)
+    {
+        && spec.init <= inv
+        && forall b, y ::
+            && |b| > 0
+            && Spec.BehaviorSatisfies(b, spec)
+            && (var x := b[|b| - 1];
+            && x in inv
+            && (x, y) in spec.next)
             ==> y in inv
     }
 
     predicate IsInvariant<A>(inv: iset<A>, spec: Spec.T<A>)
     {
-        forall b, i :: 
+        forall b, i ::
             && Spec.BehaviorSatisfies(b, spec)
             && 0 <= i < |b|
             ==> b[i] in inv
     }
 
-    lemma EstablishInvariant<A>(inv: iset<A>, spec: Spec.T<A>)
+    lemma EstablishInvariantByInduction<A>(inv: iset<A>, spec: Spec.T<A>)
         requires IsInductive(inv, spec)
         ensures  IsInvariant(inv, spec)
     {
-        forall b, i | 
-            && Spec.BehaviorSatisfies(b, spec)
-            && 0 <= i < |b|
-        ensures b[i] in inv 
+        forall b | Spec.BehaviorSatisfies(b, spec)
+        ensures forall i :: 0 <= i < |b| ==> b[i] in inv
         {
             var j := 0;
-            while j < i
-                invariant 0 <= j <= i
-                invariant b[j] in inv
+            while j < |b|
+                invariant 0 <= j <= |b|
+                invariant forall i :: 0 <= i < j ==> b[i] in inv
+            {
+                if j != 0 {
+                    assert (b[j-1], b[j]) in spec.next;
+                }
+
+                j := j + 1;
+            }
+        }
+    }
+
+    lemma EstablishInvariantByInductionInReachable<A>(inv: iset<A>, spec: Spec.T<A>)
+        requires IsInductiveInReachable(inv, spec)
+        ensures IsInvariant(inv, spec)
+    {
+        forall b | Spec.BehaviorSatisfies(b, spec)
+        ensures forall i :: 0 <= i < |b| ==> b[i] in inv
+        {
+            var j := 0;
+            while j < |b|
+                invariant 0 <= j <= |b|
+                invariant Spec.BehaviorSatisfies(b[..j], spec)
+                invariant forall i :: 0 <= i < j ==> b[i] in inv
             {
                 j := j + 1;
             }
         }
+    }
+
+    lemma InvariantImplies<A>(inv1: iset<A>, inv2: iset<A>, spec: Spec.T<A>)
+        requires IsInvariant(inv1, spec)
+        requires inv1 <= inv2
+        ensures IsInvariant(inv2, spec)
+    {}
+
+    lemma InvariantTrueInitially<A>(inv: iset<A>, spec: Spec.T<A>)
+        requires IsInvariant(inv, spec)
+        ensures spec.init <= inv
+    {
+        forall x | x in spec.init
+            ensures x in inv
+        {
+            var b := [x];
+            assert Spec.BehaviorSatisfies(b, spec);
+        }
+    }
+
+    function InvariantAndReachable<A>(inv: iset<A>, spec: Spec.T<A>): iset<A>
+    {
+        iset a: A, b |
+            && a in inv
+            && |b| > 0
+            && Spec.BehaviorSatisfies(b, spec)
+            && a == b[|b|-1]
+        :: a
+    }
+
+    lemma InvariantAndReachableIsInvariant<A>(inv: iset<A>, spec: Spec.T<A>)
+        requires IsInvariant(inv, spec)
+        ensures IsInvariant(InvariantAndReachable(inv, spec), spec)
+    {
+        forall a | a in spec.init
+            ensures a in InvariantAndReachable(inv, spec)
+        {
+            var b := [a];
+            assert Spec.BehaviorSatisfies(b, spec) && b[0] in inv;
+        }
+
+        forall b, y |
+            && |b| > 0
+            && Spec.BehaviorSatisfies(b, spec)
+            && (var x := b[|b| - 1];
+            && x in InvariantAndReachable(inv, spec)
+            && (x, y) in spec.next)
+            ensures y in InvariantAndReachable(inv, spec)
+        {
+            var b' := b + [y];
+            assert Spec.BehaviorSatisfies(b', spec) && b'[|b'| - 1] in inv;
+        }
+
+        EstablishInvariantByInductionInReachable(InvariantAndReachable(inv, spec), spec);
     }
 }
 
@@ -112,20 +221,76 @@ module ConjoinInvariant {
     import Invariants
     import Simulation
 
+    function ConjoinInvariantToInit<A>(init: iset<A>, inv: iset<A>): iset<A>
+    {
+        init * inv
+    }
+
+    function ConjoinInvariantToNext<A>(next: iset<(A, A)>, inv: iset<A>): iset<(A, A)>
+    {
+        iset a1, a2 | (a1, a2) in next && a1 in inv && a2 in inv :: (a1, a2)
+    }
+
     function ConjoinInvariantToSpec<A>(spec: Spec.T<A>, inv: iset<A>): Spec.T<A>
     {
-        spec
+        Spec.Make(ConjoinInvariantToInit(spec.init, inv), ConjoinInvariantToNext(spec.next, inv))
     }
 
     function ConjoinInvariantSimulation<A>(spec: Spec.T<A>, inv: iset<A>): iset<(A, A)>
     {
-        iset a | a in inv :: (a, a)
+        iset a, b |
+            a in inv && Spec.BehaviorSatisfies(b, spec) && |b| > 0 && a == b[|b| - 1] :: (a, a)
     }
 
     function ConjoinInvariantRequest<A>(spec: Spec.T<A>, inv: iset<A>): Simulation.Request<A, A>
     {
-        Simulation.Request(spec, ConjoinInvariantToSpec(spec, inv), ConjoinInvariantSimulation(spec, inv))
+        Simulation.Request(
+            spec,
+            ConjoinInvariantToSpec(spec, inv),
+            ConjoinInvariantSimulation(spec, inv)
+            )
     }
+
+    lemma ConjoinInitSimulation<A>(spec: Spec.T<A>, inv: iset<A>)
+        requires Invariants.IsInvariant(inv, spec)
+        ensures (var req := ConjoinInvariantRequest(spec, inv);
+            Simulation.InitDiagram(req))
+    {
+        var req := ConjoinInvariantRequest(spec, inv);
+        forall l | l in req.lspec.init
+            ensures exists h ::
+                h in req.hspec.init && (l, h) in req.sim_rel
+        {
+            Invariants.InvariantTrueInitially(inv, spec);
+            var b := [l];
+            assert Spec.BehaviorSatisfies(b, spec);
+            assert l in req.hspec.init && (l, l) in req.sim_rel;
+        }
+
+    }
+
+    lemma ConjoinNextSimulation<A>(spec: Spec.T<A>, inv: iset<A>)
+        requires Invariants.IsInvariant(inv, spec)
+        ensures (var req := ConjoinInvariantRequest(spec, inv);
+            Simulation.NextDiagram(req))
+    {
+        var req := ConjoinInvariantRequest(spec, inv);
+
+        forall l, l', h |
+            && (l, l') in req.lspec.next
+            && (l, h) in req.sim_rel
+        ensures
+            && (h, l') in req.hspec.next
+            && (l', l') in req.sim_rel
+        {
+            var b :| Spec.BehaviorSatisfies(b, spec) && |b| > 0 && l == b[|b| - 1];
+            var b' := b + [l'];
+            Spec.ExtendBehavior(spec, b, l');
+
+            assert b'[|b'| - 1] in inv;
+        }
+    }
+
 
     lemma ConjoinInvariantToSpecSimulation<A>(spec: Spec.T<A>, inv: iset<A>)
         returns (req: Simulation.Request<A, A>)
@@ -134,14 +299,8 @@ module ConjoinInvariant {
         ensures Simulation.ValidRequest(req)
     {
         req := ConjoinInvariantRequest(spec, inv);
-        forall l | l in req.lspec.init 
-            ensures exists h :: 
-                && h in req.hspec.init
-                && (l, h) in req.sim_rel
-        {
-            var b := [l];
-            assert Spec.BehaviorSatisfies(b, spec);
-            assert b[0] in inv;
-        }
+
+        ConjoinInitSimulation(spec, inv);
+        ConjoinNextSimulation(spec, inv);
     }
 }
